lib/misc.v
@@ -10,17 +10,16 @@ Definition oloc_to_val (ol: option loc) : val :=
   end.
 
 Local Open Scope Z.
-Definition node_rep : Type := Z * option loc * bool * val.
-Definition node_key (n: node_rep) : Z := n.1.1.1.
-Definition node_next (n: node_rep) : option loc := n.1.1.2.
-Definition node_mark (n: node_rep) : bool := n.1.2.
+Definition node_rep : Type := Z * option loc * val.
+Definition node_key (n: node_rep) : Z := n.1.1.
+Definition node_next (n: node_rep) : option loc := n.1.2.
 Definition node_lock (n: node_rep) : val := n.2.
 
 Definition node_lt (x y: node_rep) : Prop := 
   node_key x < node_key y.
 
 Definition rep_to_node (n: node_rep) : val :=
-  (#(node_key n), oloc_to_val (node_next n), #(node_mark n), (node_lock n)).
+  (#(node_key n), oloc_to_val (node_next n), (node_lock n)).
 
 Definition key_equiv (S: gset node_rep) (S_keys: gset Z) :=
   Permutation (elements S_keys) (map node_key (elements S)).
